separate traversal proofs

templates/lockfree/skiplist_v0.v
@@ -102,16 +102,21 @@ Node local info:
 
 Definition K := Z.
 
+Definition esT : Type := gmap Node (gset K).
+
 Definition flowUR := authR (multiset_flowint_ur K).
 Definition auth_keysetUR := authUR $ (keysetUR K).
+Definition auth_setnodeUR := authUR $ (gsetUR Node).
 
 Class skG Σ := SK {
                   sk_flowG :> inG Σ flowUR;
                   sk_auth_keysetG :> inG Σ auth_keysetUR;
+                  sk_auth_setnodeG :> inG Σ auth_setnodeUR;
                  }.
                  
 Definition skΣ : gFunctors :=
-  #[ GFunctor flowUR;  GFunctor auth_keysetUR ].
+  #[ GFunctor flowUR;  GFunctor auth_keysetUR;
+     GFunctor auth_setnodeUR ].
   
 Instance subG_skΣ {Σ} : subG skΣ Σ → skG Σ.
 Proof. solve_inG. Qed.
@@ -120,126 +125,131 @@ Section skiplist_v0.
   Context {Σ} `{!heapGS Σ, !skG Σ}.
   Notation iProp := (iProp Σ).
   
-  Parameter node : Node → bool → (multiset_flowint_ur K) → (gset K) → iProp.
+  Parameter node : Node → bool → esT → (gset K) → iProp.
   Parameter node_timeless_proof : ∀ r n es V, Timeless (node r n es V).
   Global Instance node_timeless r n es V: Timeless (node r n es V).
   Proof. apply node_timeless_proof. Qed.  
 
+  Parameter Mark : snapshot → Node → bool.
+  Parameter ES : snapshot → Node → esT.
   Parameter PC : snapshot → Node → gset K.
-  Parameter mark : snapshot → Node → bool.
-  Parameter gintf : snapshot → (multiset_flowint_ur K).
-  Parameter intf : snapshot → Node → (multiset_flowint_ur K).
-  Parameter γ_I : snapshot → gname.
-  Parameter γ_ks : snapshot → gname.
+  Parameter GFI : snapshot → (multiset_flowint_ur K).
+  Parameter FI : snapshot → Node → (multiset_flowint_ur K).
   Parameter FP : snapshot → gset Node.
 
   Definition Cont (s: snapshot) (n: Node) : gset K :=
-    if decide (mark s n) then ∅ else PC s n.
+    if decide (Mark s n) then ∅ else PC s n.
 
   Parameter out_set : multiset_flowint_ur K → gset K.
-  Parameter out_map : multiset_flowint_ur K → gmap Node (gset K).
-  Parameter keyset : multiset_flowint_ur K → gset K.
+  (* out_es es := ⋃_n es !!! n *)
+  Parameter out_es : esT → gset K.
+  Parameter keyset : multiset_flowint_ur K → gset K. 
     
-  (** data structure specific inv *)  
+  (** data structure specific inv *)
 
-  Definition node_local_pure s n : iProp :=
-      ⌜¬ (mark s n) → out_set (intf s n) ⊆ inset K (intf s n) n⌝
-    ∗ ⌜Cont s n ⊆ keyset (intf s n)⌝
-    ∗ ⌜mark s n → out_set (intf s n) ≠ ∅⌝.
+  Definition globalRes γ_I γ_fp γ_ks s : iProp :=
+      own γ_I (● (GFI s)) 
+    ∗ own γ_fp (● FP s) 
+    ∗ own γ_ks (● prod (KS, abs s)).
+  
+  Definition outflow_constraint (In: multiset_flowint_ur K) (esn: esT) : Prop := True.
 
+  Definition node_inv_pure s n : iProp :=
+      ⌜¬ (Mark s n) → out_set (FI s n) ⊆ inset K (FI s n) n⌝
+    ∗ ⌜Cont s n ⊆ keyset (FI s n)⌝
+    ∗ ⌜Mark s n → out_set (FI s n) ≠ ∅⌝
+    ∗ ⌜outflow_constraint (FI s n) (ES s n)⌝ .
+
+  Definition node_inv γ_I γ_ks s n : iProp :=
+      node n (Mark s n) (ES s n) (PC s n)
+    ∗ own γ_I (◯ (FI s n))
+    ∗ own γ_ks (◯ prod (keyset (FI s n), Cont s n))
+    ∗ node_inv_pure s n.   
+(*
   Definition node_local_inv s n : iProp :=
       own (γ_I s) (◯ intf s n) 
     ∗ own (γ_ks s) (◯ prod (keyset (intf s n), Cont s n))
     ∗ node_local_pure s n.
-
+*)
   Definition per_tick_inv r s : iProp := 
-      own (γ_I s) (● (gintf s)) ∗ own (γ_ks s) (● prod (KS, abs s))
-    ∗ ⌜inset K (intf s r) r = KS⌝ ∗ ⌜out_set (intf s r) = KS⌝
-    ∗ ⌜¬ mark s r⌝
-    ∗ [∗ set] n ∈ (FP s), node_local_inv s n.
+      ⌜inset K (FI s r) r = KS⌝ ∗ ⌜out_set (FI s r) = KS⌝
+    ∗ ⌜¬ Mark s r⌝
+    ∗ [∗ set] n ∈ (FP s), node_inv_pure s n.
     
   Definition transition_inv s s' : Prop :=
-      (∀ n, n ∈ FP s → mark s n → out_map (intf s n) = out_map (intf s' n))
-    ∧ (∀ n, n ∈ FP s → mark s n → mark s' n)
-    ∧ (∀ n, n ∈ FP s → 
-        (¬ mark s n ∧ mark s' n ∧ out_set (intf s n) ≠ out_set (intf s' n)) ∨
-        (mark s n ∧ mark s' n ∧ out_set (intf s n) = out_set (intf s' n)))
+      (∀ n, n ∈ FP s → Mark s n → ES s' n = ES s n)
+    ∧ (∀ n, n ∈ FP s → Mark s n → Mark s' n)
+    ∧ (∀ n, n ∈ FP s → ¬ Mark s n → Mark s' n → ES s n ≠ ES s' n)
     ∧ (∀ n, n ∈ FP s → PC s n = PC s' n)
     ∧ (FP s ⊆ FP s').
-  
-  (** resources inv *)
 
-  Definition nodeFull s n : iProp :=
-    ∃ m In pc,
-      node n m In pc
-    ∗ ⌜m = mark s n⌝ ∗ ⌜In = intf s n⌝ ∗ ⌜pc = PC s n⌝  
-    ∗ own (γ_I s) (◯ In)
-    ∗ own (γ_ks s) (◯ prod (keyset In, Cont s n)).   
-  
-  Definition resources s : iProp :=
-      [∗ set] n ∈ FP s, nodeFull s n. 
-        
-  Definition skiplist_inv r (M: gmap nat snapshot) 
-    (T: nat) (s: snapshot): iProp :=
-      ([∗ set] t ∈ dom M, per_tick_inv r (M !!! t))
+  Definition skiplist_inv γ_I γ_fp γ_ks r (M: gmap nat snapshot) 
+    (T: nat) (s: snapshot) : iProp :=
+      globalRes γ_I γ_fp γ_ks s
+    ∗ ([∗ set] n ∈ FP s, node_inv γ_I γ_ks s n)
+    ∗ ([∗ set] t ∈ dom M, per_tick_inv r (M !!! t))
     ∗ ⌜∀ t, 0 ≤ t < T → transition_inv (M !!! t) (M !!! (t+1)%nat)⌝
-    ∗ ⌜transition_inv (M !!! T) s⌝
-    ∗ ([∗ set] n ∈ FP s, nodeFull s n).
+    ∗ ⌜transition_inv (M !!! T) s⌝.
     
-  Instance skiplist_inv_timeless r M T s : Timeless (skiplist_inv r M T s).
+  Instance skiplist_inv_timeless γ_I γ_fp γ_ks r M T s : 
+    Timeless (skiplist_inv γ_I γ_fp γ_ks r M T s).
   Proof.
   Admitted.     
     
   (** Helper functions specs *)
     
   Parameter inContents_spec : ∀ (k: K) (n: Node),
-     ⊢ (<<< ∀∀ m In pc, node n m In pc >>>
+     ⊢ (<<< ∀∀ m es pc, node n m es pc >>>
            inContents #n #k @ ⊤
        <<< ∃∃ (v: bool),
-              node n m In pc ∗ ⌜v ↔ k ∈ pc⌝,
+              node n m es pc ∗ ⌜v ↔ k ∈ pc⌝,
               RET #v >>>)%I.
 
   Parameter findNext_spec : ∀ (k: K) (n: Node),
-     ⊢ (<<< ∀∀ m In pc, node n m In pc >>>
+     ⊢ (<<< ∀∀ m es pc, node n m es pc >>>
            findNext #n #k @ ⊤
-       <<< ∃∃ (succ: bool) (n': Node),
-              node n m In pc
-            ∗ (match succ with true => ⌜k ∈ outset K In n'⌝ 
-                             | false => ⌜k ∉ out_set In⌝ end),
-              RET (match succ with true => (#m, SOMEV #n') 
-                                 | false => (#m, NONEV) end)  >>>)%I.
+       <<< ∃∃ (success: bool) (n': Node),
+              node n m es pc
+            ∗ (match success with true => ⌜k ∈ es !!! n'⌝ 
+                                | false => ⌜k ∉ out_es es⌝ end),
+              RET (match success with true => (#m, SOMEV #n') 
+                                    | false => (#m, NONEV) end)  >>>)%I.
+                                 
+  Definition edgset_update es k curr succ : esT :=
+   <[ succ := (es !!! succ) ∪ {[k]} ]>
+    (<[ curr := (es !!! curr) ∖ {[k]} ]> es).
 
-  Parameter try_constraint_trav_spec : ∀ (k: K) (p c s: Node),
-     ⊢ (<<< ∀∀ mp Ip pcp, node p mp Ip pcp >>>
-           try_constraint #p #c #s @ ⊤
-       <<< ∃∃ (succ: bool) Ip',
-              node p mp Ip' pcp
-            ∗ (match succ with true => ⌜mp = false⌝ ∗ ⌜k ∈ (out_map Ip) !!! c⌝
-                                     ∗ ⌜k ∈ (out_map Ip') !!! s⌝ 
-                             | false => ⌜mp = true ∨ k ∉ (out_map Ip) !!! c⌝
-                                      ∗ ⌜Ip' = Ip⌝ end),
-              RET (match succ with true => SOMEV #() 
-                                 | false => NONEV end)  >>>)%I.
+  Parameter try_constraint_trav_spec : ∀ (k: K) (pred curr succ: Node),
+     ⊢ (<<< ∀∀ m es pc, node pred m es pc >>>
+           try_constraint #pred #curr #succ @ ⊤
+       <<< ∃∃ (success: bool) es',
+              node pred m es' pc
+            ∗ (match success with true => ⌜m = false⌝ ∗ ⌜k ∈ es !!! curr⌝
+                                          ∗ ⌜es' = edgset_update es k curr succ⌝ 
+                                | false => ⌜m = true ∨ k ∉ es !!! curr⌝
+                                           ∗ ⌜es' = es⌝ end),
+              RET (match success with true => SOMEV #() 
+                                    | false => NONEV end)  >>>)%I.
 
-  Parameter createNode_spec : ∀ (k: K) (c: Node),
+  Parameter createNode_spec : ∀ (k: K) (n: Node),
      ⊢ ({{{ True }}}
-           createNode #k #c
-       {{{ (e: Node) em Ie pce, RET #e;
-              node e em Ie pce
-            ∗ ⌜k ∈ pce⌝
-            ∗ ⌜k ∈ outset K Ie c⌝ }}})%I.
+           createNode #k #n
+       {{{ e m es pc, RET #e;
+              node e m es pc
+            ∗ ⌜k ∈ pc⌝
+            ∗ ⌜k ∈ es !!! n⌝ }}})%I.
 
-  Parameter try_constraint_insert_spec : ∀ (k: K) (p c e: Node),
-     ⊢ (<<< ∀∀ mp Ip pcp, node p mp Ip pcp >>>
-           try_constraint #p #c #e @ ⊤
-       <<< ∃∃ (succ: bool) Ip',
-              node p mp Ip' pcp
-            ∗ (match succ with true => ⌜mp = false⌝ ∗ ⌜k ∈ (out_map Ip) !!! c⌝
-                                     ∗ ⌜k ∈ (out_map Ip') !!! e⌝ 
-                             | false => ⌜mp = true ∨ k ∉ (out_map Ip) !!! c⌝
-                                      ∗ ⌜Ip' = Ip⌝ end),
-              RET (match succ with true => SOMEV #() 
-                                 | false => NONEV end)  >>>)%I.
+  Parameter try_constraint_insert_spec : ∀ (k: K) (pred curr entry: Node),
+     ⊢ (<<< ∀∀ m es pc, node pred m es pc >>>
+           try_constraint #pred #curr #entry @ ⊤
+       <<< ∃∃ (success: bool) es',
+              node pred m es' pc
+            ∗ (match success with true => ⌜m = false⌝ ∗ ⌜k ∈ es !!! curr⌝
+                                          ∗ ⌜es' = edgset_update es k curr entry⌝ 
+                                | false => ⌜m = true ∨ k ∉ es !!! curr⌝
+                                           ∗ ⌜es' = es⌝ end),
+              RET (match success with true => SOMEV #() 
+                                    | false => NONEV end)  >>>)%I.
 
 
 
