templates/lockfree/skiplist_v0_traverse.v
@@ -1,0 +1,274 @@
+(* Herlihy Skiplist with a single level : Search *)
+
+From iris.algebra Require Import excl auth cmra gmap agree gset numbers.
+From iris.algebra.lib Require Import dfrac_agree.
+From iris.heap_lang Require Export notation locations lang.
+From iris.base_logic.lib Require Export invariants.
+From iris.program_logic Require Export atomic.
+From iris.proofmode Require Import tactics.
+From iris.heap_lang Require Import proofmode par.
+From iris.heap_lang.lib Require Import nondet_bool.
+From iris.bi.lib Require Import fractional.
+Set Default Proof Using "All".
+From iris.bi.lib Require Import fractional.
+Require Export skiplist_v0.
+
+Section skiplist_v0_traverse.
+
+  Context {Σ} `{!heapGS Σ, !dsG Σ, !skG Σ}.
+  Notation iProp := (iProp Σ).
+
+  (** Proofs *)
+(*
+  Lemma test γ (N: gset nat) (S: gset proph_id) (F: nat → gset proph_id) :
+    own γ (● S) ∗ ([∗ set] n ∈ N, own γ (◯ (F n))) -∗ 
+      own γ (● S) ∗ ([∗ set] n ∈ N, own γ (◯ (F n))) ∗ ⌜∀ n, n ∈ N → F n ⊆ S⌝.
+  Proof.
+    iInduction N as [| n N] "IH" using set_ind_L.
+    - iIntros "(HS & Hstar)". iFrame. iPureIntro. intros n Hn; set_solver.
+    - iIntros "(HS & Hstar)".
+      rewrite (big_sepS_insert _ N n); last by eauto.
+      iDestruct "Hstar" as "(Hn & Hstar)".
+      iAssert (⌜F n ⊆ S⌝)%I as "%HFn".
+      { admit. }
+      iCombine "HS Hstar" as "H'".
+      iDestruct ("IH" with "H'") as "(HS & star & %IH)".
+      iFrame. iPureIntro. 
+      intros n'. rewrite elem_of_union.
+      intros [Hn | Hn].
+      + assert (n' = n) as -> by set_solver.
+        try done.
+      + apply IH; try done.
+  Admitted.
+      
+  
+  Lemma temporal_interpolation_test1 (M : gmap nat nat) (T: nat) (FP: nat → gset K) :
+      (∀ t, 0 ≤ t < T → FP (M !!! t) ⊆ FP (M !!! (t+1)%nat)) →
+        (∀ t1 t2, 0 ≤ t1 ≤ t2 → t2 < T → FP (M !!! t1) ⊆ FP (M !!! t2)).
+  Proof.
+    intros Hcons. induction t1.
+    - induction t2.
+      + intros; try done.
+      + intros Ht2 Ht2_T.
+        assert (FP (M !!! 0) ⊆ FP (M !!! t2)) as H'.
+        { apply IHt2. lia. lia. }
+        assert (FP (M !!! t2) ⊆ FP (M !!! S t2)) as H''.
+        { assert (t2 + 1 = S t2) as <- by lia.
+          apply Hcons. lia. }
+        clear -H' H''. set_solver.
+    - induction t2.
+      + intros H'. exfalso; lia.
+      + intros Ht1 Ht2_T.
+        assert (FP (M !!! t2) ⊆ FP (M !!! S t2)) as H'.
+        { assert (t2 + 1 = S t2) as <- by lia.
+          apply Hcons. lia. }
+        destruct (decide (S t1 <= t2)).
+        * assert (FP (M !!! S t1) ⊆ FP (M !!! t2)) as H''.
+          { apply IHt2; try lia. }
+          clear -H' H''. set_solver.
+        * assert (t1 = t2) by lia.
+          by subst t1.
+  Qed.
+  
+  Lemma temporal_interpolation_test2 (M : gmap nat nat) 
+    (T t1 t2: nat) (Mark: nat → bool) :
+      (∀ t, 0 ≤ t < T → Mark (M !!! t) = true → Mark (M !!! S t) = true) →
+        Mark (M !!! t1) = false → Mark (M !!! t2) = true → t1 ≤ t2 ≤ T →
+        (∃ t, t1 ≤ t < t2 ∧ Mark (M !!! t) = false ∧ Mark (M !!! S t) = true).
+  Proof.
+    intros Htrans; induction t1; induction t2; 
+    intros Mark1 Mark2 t1_le_t2.
+    - exfalso. rewrite Mark2 in Mark1. inversion Mark1.
+    - destruct (decide (Mark (M !!! t2) = true)). 
+      + assert (0 ≤ t2 ≤ T) as H' by lia.
+        pose proof IHt2 Mark1 e H' as IHt2.
+        destruct IHt2 as [t [Ht [Mark1' Mark2']]].
+        exists t; repeat split; try (done || lia).
+      + exists t2. repeat split; try (done || lia).
+        by rewrite not_true_iff_false in n.
+    - assert (t1 = 0) as -> by lia.
+      assert (0 ≤ 0 < T) as H' by lia.
+      pose proof Htrans 0 H' Mark2 as Htrans.
+      exfalso. rewrite Htrans in Mark1. inversion Mark1.
+    - assert (t1 < t2 ∨ t1 = t2) as Hor by lia.
+      destruct Hor as [Hor | ->].
+      + destruct (decide (Mark (M !!! t2) = true)).
+        * assert (Mark (M !!! t1) = false) as H'.
+          { destruct (decide (Mark (M !!! t1) = false)); try done.
+            rewrite not_false_iff_true in n.
+            assert (0 ≤ t1 < T) as H' by lia.
+            pose proof Htrans t1 H' n as Htrans.
+            rewrite Htrans in Mark1. inversion Mark1. }
+          assert (t1 ≤ S t2 ≤ T) as H'' by lia.
+          pose proof IHt1 H' Mark2 H'' as IHt1.
+          destruct IHt1 as [t [Ht [Mark1' Mark2']]].
+          exists t; repeat split; try (done || lia).
+          assert (t1 < t ∨ t1 = t) as Hor2 by lia.
+          destruct Hor2 as [Hor2 | ->]; try lia.
+          rewrite Mark1 in Mark2'. inversion Mark2'.
+        * rewrite not_true_iff_false in n.
+          exists t2; split; try (done || lia).
+      + rewrite Mark1 in Mark2; inversion Mark2.    
+  Qed.
+*)  
+  Definition traverse_rec_inv γ_m t0 k s p c : iProp :=
+      past_state γ_m t0 s
+    ∗ ⌜p ∈ FP s⌝ ∗ ⌜c ∈ FP s⌝   
+    ∗ ⌜¬ Mark s p⌝
+    ∗ ⌜k ∈ outset K (FI s p) c⌝. 
+
+  Lemma traverse_rec_spec N γ_t γ_s γ_m γ_td γ_ght γ_I γ_fp γ_ks r 
+    γ_sy t_id t0 (k: K) s p c:
+    ⌜k ∈ KS⌝ -∗
+      css_inv N γ_t γ_s γ_m γ_td γ_ght (skiplist_inv γ_I γ_fp γ_ks r) -∗
+       thread_vars γ_t γ_ght γ_sy t_id t0 -∗  
+        traverse_rec_inv γ_m t0 k s p c -∗
+          {{{ True }}}
+            traverse_rec r #p #c #k
+          {{{ (p' c': Node) s, RET (#p', #c');
+                past_state γ_m t0 s
+              ∗ ⌜p' ∈ FP s⌝ ∗ ⌜c' ∈ FP s⌝   
+              ∗ ⌜¬ Mark s p'⌝
+              ∗ ⌜k ∈ inset K (FI s p') p'⌝
+              ∗ ⌜k ∈ outset K (FI s p') c'⌝
+              ∗ ⌜¬ Mark s c'⌝
+              ∗ ⌜k ∈ keyset (FI s c')⌝ }}}.
+  Proof.
+    iIntros "%k_in_KS #HInv #Thd". 
+    iLöb as "IH" forall (s p c). 
+    iIntros "#Tr_inv" (Φ) "!# _ Hpost".
+    wp_lam. wp_pures. awp_apply (findNext_spec); try done.
+    iInv "HInv" as (M0 T0 s0) "(>CSS & >%Habs0 & >Hist & Help & >Templ)".
+    { admit. }
+    iDestruct "Templ" as "(Hglob & Res & PT & %Trans_M0 & %Trans_s0)". 
+    iAssert (⌜c ∈ FP s0⌝)%I as %FP_c.
+    { admit. }
+    rewrite (big_sepS_delete _ (FP s0) c); last by eauto.
+    iDestruct "Res" as "((Node_c & Node_crest) & Res_rest)".
+    iAaccIntro with "Node_c".
+    { iIntros "Node_c". iModIntro. iFrame "Hpost". 
+      iNext; iExists M0, T0, s0.
+      iFrame "∗#%". 
+      rewrite (big_sepS_delete _ (FP s0) c); last by eauto. 
+      iFrame. }
+    iIntros (succ n) "(Node & Hif)".
+    destruct (Mark s0 c); destruct succ.
+    - iModIntro. iSplitR "Hpost".
+      { admit. }
+      wp_pures. awp_apply (try_constraint_trav_spec k).
+      iInv "HInv" as (M1 T1 s1) "(>CSS & >%Habs1 & >Hist & Help & >Templ)".
+      { admit. }
+      iDestruct "Templ" as "(Hglob & Res & PT & %Trans_M1 & %Trans_s1)".
+      iAssert (⌜p ∈ FP s1⌝)%I as %FP_p.
+      { admit. }
+      rewrite (big_sepS_delete _ (FP s1) p); last by eauto.
+      iDestruct "Res" as "((Node_p & Node_prest) & Res_rest)".
+      iAaccIntro with "Node_p".
+      { iIntros "Node_p". admit. }
+      iIntros (succ es') "(Node_p & Hif)".
+      destruct succ.
+      + iDestruct "Hif" as %(mark_p_false & k_in_p2c & Def_es').
+        admit.
+      + iModIntro. iSplitR "Hpost".
+        { admit. } 
+        wp_pures.
+        admit.
+    - iModIntro. iSplitR "Hpost".
+      { admit. }
+      wp_pures. iExFalso. admit.
+    - iModIntro. iSplitR "Hpost".
+      { admit. } 
+      wp_pures. admit.
+  Admitted.
+
+  Lemma traverse_spec N γ_t γ_s γ_m γ_td γ_ght γ_I γ_fp γ_ks r γ_sy t_id t0 (k: K) :
+    ⌜k ∈ KS⌝ -∗
+      css_inv N γ_t γ_s γ_m γ_td γ_ght (skiplist_inv γ_I γ_fp γ_ks r) -∗
+       thread_vars γ_t γ_ght γ_sy t_id t0 -∗  
+        {{{ True }}}
+           traverse r #k
+        {{{ (p c: Node) s, RET (#p, #c); 
+              past_state γ_m t0 s
+            ∗ ⌜p ∈ FP s⌝ ∗ ⌜c ∈ FP s⌝   
+            ∗ ⌜¬ Mark s p⌝
+            ∗ ⌜k ∈ inset K (FI s p) p⌝
+            ∗ ⌜k ∈ outset K (FI s p) c⌝
+            ∗ ⌜¬ Mark s c⌝
+            ∗ ⌜k ∈ keyset (FI s c)⌝ }}}.
+  Proof.
+    iIntros "%k_in_KS #HInv #Thd". iIntros (Φ) "!# _ Hpost".
+    wp_lam. awp_apply (findNext_spec); try done.
+    iInv "HInv" as (M0 T0 s0) "(>CSS & >%Habs0 & >Hist & Help & >Templ)".
+    { admit. }
+    iDestruct "Templ" as "(Hglob & Res & PT & %Trans_M0 & %Trans_s0)". 
+    iAssert (⌜r ∈ FP s0⌝)%I as %FP_r0.
+    { admit. }
+    rewrite (big_sepS_delete _ (FP s0) r); last by eauto.
+    iDestruct "Res" as "((Node_r & Node_rrest) & Res_rest)".
+    iAaccIntro with "Node_r".
+    { iIntros "Node_r". iModIntro. iFrame "Hpost". 
+      iNext; iExists M0, T0, s0.
+      iFrame "∗#%". 
+      rewrite (big_sepS_delete _ (FP s0) r); last by eauto. 
+      iFrame. }
+    iIntros (succ n) "(Node & Hif)".
+    destruct succ; last first.
+    - iAssert (⌜k ∉ KS⌝)%I as %k_notin_KS.
+      { iAssert (⌜T0 ∈ dom M0⌝)%I as %t_in_M0.
+        { admit. }
+        rewrite (big_sepS_delete _ (dom M0) T0); last by eauto.
+        iDestruct "PT" as "(PT_T0 & PT_rest)".
+        iAssert (per_tick_inv r (s0))%I with "[PT_T0]" as "PT_T0".
+        { admit. }
+        iDestruct "PT_T0" as "(Ins_r & Out_r & Mark_r & Hbig_star)".
+        iDestruct "Hif" as %Hif.
+        iDestruct "Out_r" as %Out_r.
+        iDestruct "Node_rrest" as "(_&_&%H'&_)".
+        iPureIntro. rewrite <-H' in Out_r.
+        by rewrite Out_r in Hif. }
+      iClear "∗#". clear -k_in_KS k_notin_KS. exfalso; try done.
+    - iModIntro.
+      iAssert (past_state γ_m t0 s0)%I as "#Hist_s0".
+      { admit. }
+      iAssert (⌜n ∈ FP s0⌝)%I as %FP_n.
+      { admit. }
+      iAssert (⌜T0 ∈ dom M0⌝)%I as %T0_in_M0.
+      { admit. }
+      rewrite (big_sepS_delete _ (dom M0) T0); last by eauto.
+      iDestruct "PT" as "(PT_T0 & PT_rest)".
+      iAssert (per_tick_inv r (s0))%I with "[PT_T0]" as "PT_T0".
+      { admit. }
+      iDestruct "PT_T0" as "(HI & HKS & %Ins_r & %Out_r 
+          & %Mark_r & Hbig_star)".
+      iAssert (⌜k ∈ inset K (intf s0 r) r⌝)%I as %k_in_Insr.
+      { iPureIntro. by rewrite Ins_r. }
+      iDestruct "Hif" as %k_in_Outr.
+      iAssert (⌜n ≠ r⌝)%I as "%n_neq_r".
+      { admit. }
+      iAssert (⌜n ∈ FP s0 ∖ {[r]}⌝)%I as "%".
+      { clear -FP_n n_neq_r. iPureIntro; set_solver. } 
+      rewrite (big_sepS_delete _ (FP s0 ∖ {[r]}) n); last by eauto.
+      iDestruct "Res_rest" as "(NodeFull_n & Res_rest)".
+      iDestruct "NodeFull_n" as (mn In pcn) "(Node_n & Node_n_rest)".
+      iAssert (⌜Ir = intf s0 r⌝)%I as %HIr.
+      { by iDestruct "Node_rest" as "(_&%&_)". }
+      rewrite HIr in k_in_Outr.
+      iAssert (⌜k ∈ inset K (intf s0 n) n⌝)%I as %k_in_Insn.
+      { admit. }
+      iAssert (traverse_rec_inv γ_m t0 k s0 r n)%I as "#Tr_inv".
+      { iFrame "#%". }
+      iSplitR "Hpost". 
+      { iNext. iExists M0, T0, s0.
+        iFrame "∗#%".
+        rewrite (big_sepS_delete _ (dom M0) T0); last by eauto.
+        iFrame. iSplitL "HI HKS Hbig_star".
+        { admit. }
+        rewrite (big_sepS_delete (nodeFull s0) (FP s0) r); last by eauto.
+        rewrite (big_sepS_delete _ (FP s0 ∖ {[r]}) n); last by eauto.
+        iFrame. iSplitL "Node Node_rest". 
+        iExists mr, Ir, pcr. iFrame.
+        iExists mn, In, pcn. iFrame. }   
+      wp_pures. wp_apply traverse_rec_spec; try done.
+  Admitted.
+
+End skiplist_v0_traverse.
